IL/BlockType.v
@@ -1,0 +1,48 @@
+Require Import AllInRel List Map Env AutoIndTac MoreList IL.
+
+Set Implicit Arguments.
+
+Class BlockType X := {
+                      block_n : X -> nat;
+                      block_Z : X -> list var
+                    }.
+
+Instance block_type_I : BlockType (I.block) :=
+  {
+    block_n := I.block_n;
+    block_Z := I.block_Z
+  }.
+
+Instance block_type_F : BlockType (F.block) :=
+  {
+    block_n := F.block_n;
+    block_Z := F.block_Z
+  }.
+
+
+Lemma mkBlocks_I_less
+  : forall (F : list (params * stmt)) (n k : nat) (b : I.block),
+    get (mapi_impl I.mkBlock k F) n b -> I.block_n b <= k + length F - 1.
+Proof.
+  intros; inv_get. simpl. eapply get_range in H. omega.
+Qed.
+
+Lemma mkBlock_I_i F
+  : forall i b, get (mapi I.mkBlock F) i b -> i = I.block_n b.
+Proof.
+  intros; inv_get; eauto.
+Qed.
+
+
+Lemma mkBlocks_F_less
+  : forall E (F : list (params * stmt)) (n k : nat) (b : F.block),
+    get (mapi_impl (F.mkBlock E) k F) n b -> F.block_n b <= k + length F - 1.
+Proof.
+  intros; inv_get. simpl. eapply get_range in H. omega.
+Qed.
+
+Lemma mkBlock_F_i E F
+  : forall i b, get (mapi (F.mkBlock E) F) i b -> i = F.block_n b.
+Proof.
+  intros; inv_get; eauto.
+Qed.
