IL/ILN_IL.v
@@ -1,0 +1,340 @@
+Require Import List.
+Require Import Util Var Val Exp Env Map CSet AutoIndTac IL.
+Require Import Bisim BisimTactics Infra.Status Pos ILN InRel Sawtooth.
+
+Set Implicit Arguments.
+Unset Printing Records.
+
+Instance block_type_I : BlockType (I.block) :=
+  {
+    block_n := I.block_f;
+    block_Z := I.block_Z
+  }.
+
+
+Fixpoint labIndices (symb: list var) (s:nstmt) : status stmt :=
+  match s with
+    | nstmtLet x e s => sdo s' <- (labIndices symb s); Success (stmtLet x e s')
+    | nstmtIf x s1 s2 =>
+      sdo s1' <- (labIndices symb s1);
+      sdo s2' <- (labIndices symb s2);
+      Success (stmtIf x s1' s2')
+    | nstmtApp l Y =>
+      sdo f <- option2status (pos symb l 0) "labIndices: Undeclared function" ; Success (stmtApp (LabI f) Y)
+    | nstmtReturn x => Success (stmtReturn x)
+    | nstmtExtern x f Y s =>
+      sdo s' <- (labIndices symb s); Success (stmtExtern x f Y s')
+    | nstmtFun F s2 =>
+      let fl := List.map (fst ∘ fst) F in
+      sdo F' <- smap (fun (fZs:var*params*nstmt) => sdo s <- labIndices (fl ++ symb) (snd fZs);
+                    Success (snd (fst fZs), s)) F;
+      sdo s2' <- labIndices (fl++symb) s2;
+      Success (stmtFun F' s2')
+  end.
+
+Lemma labIndices_freeVars ilin s L
+: labIndices L ilin = Success s
+  -> freeVars ilin = IL.freeVars s.
+Proof.
+  revert_except ilin.
+  sind ilin; destruct ilin; simpl in *; intros; monadS_inv H; simpl.
+  - erewrite IH; eauto with cset.
+  - erewrite IH; eauto.
+    erewrite IH; eauto.
+  - reflexivity.
+  - reflexivity.
+  - erewrite IH; eauto.
+  - erewrite IH; eauto.
+    f_equal. f_equal.
+    exploit smap_length; eauto.
+    erewrite map_ext_get_eq; eauto with len.
+    intros; inv_get.
+    eapply smap_spec in EQ; eauto. destruct EQ; dcr.
+    monadS_inv H3; get_functional; simpl in *.
+    erewrite IH; eauto.
+Qed.
+
+Lemma pos_drop_eq symb (l:lab) x
+: pos symb l 0 = Some x
+  -> drop x symb = l::tl (drop x symb).
+Proof.
+  general induction symb.
+  unfold pos in H; fold pos in H.
+  cases in H; simpl; eauto.
+  - inv COND; eauto.
+  - destruct x.
+    + exfalso. exploit (pos_ge _ _ _ H); eauto. omega.
+    + simpl. erewrite IHsymb; eauto.
+      eapply (pos_sub 1); eauto.
+Qed.
+
+Lemma pos_plus symb (f:lab) n i
+: pos symb f 0 = Some (n + i)
+  -> pos (drop n symb) f 0 = Some i.
+Proof.
+  general induction n; simpl; eauto.
+  destruct symb; simpl.
+  + inv H.
+  + eapply IHn; eauto. simpl in H; cases in H.
+    * inv H.
+    * eapply (pos_sub 1); eauto.
+Qed.
+
+Require Import InRel Sawtooth.
+
+Lemma mkBlocks_I_less
+      : forall F' L F (n k : nat) (b : I.block),
+          get (mapi_impl (I.mkBlock L F') k F) n b -> I.block_f b <= k + length F - 1.
+Proof.
+  intros. general induction F; simpl in *.
+  - inv H; simpl in *; try omega.
+  - inv H; simpl in *; try omega.
+    eapply IHF in H4; eauto. omega.
+Qed.
+
+Inductive lab_approx : list var -> list IL.I.block -> list I.block -> Prop :=
+  Lai symb L' LB
+    (LEQ: forall f f' Lb F i,
+            get LB i (I.blockI Lb F f')
+            -> get symb i f
+            -> (*lab_approx (drop (i-f') symb) (drop (i-f') L')  (drop (i-f') LB)
+              /\ *) (forall f blk, Lb f = Some blk -> f ∉ of_list (List.map (fst ∘ fst) F)
+                          -> exists j, pos (drop (i - f') symb) f 0 = Some j /\
+                                 get (drop (i - f') LB) j blk)
+              /\ (forall f i' k, pos (drop (i-f' + length F) symb) f k = Some i' -> exists blk, Lb f = Some blk)
+              /\ (exists Z s, get F f' (f, Z, s))
+              /\ (forall fn fb Z s, get F fn (fb,Z,s) ->
+                              (forall b n, n < fn -> get F n b -> fst (fst b) <> fb) ->
+                              exists s', get (drop (i-f') L') fn
+                                        (IL.I.blockI Z s' fn)
+                                    /\ labIndices (drop (i-f') symb) s
+                                      = Success s'
+                                    /\ pos (drop (i-f') symb) fb 0 = Some fn)
+              /\ (exists symb', drop (i-f') symb
+                          = (List.map (fst ∘ fst) F ++ symb')%list)
+              /\ (exists LB', drop (i-f') LB
+                          = (mapi (I.mkBlock Lb F) F ++ LB')%list)
+              /\ i >= f'
+
+    )
+    (ST:sawtooth LB)
+ : lab_approx symb L' LB.
+
+Lemma lab_approx_drop symb L' LB
+: forall f f' Lb F i,
+    get LB i (I.blockI Lb F f')
+    -> get symb i f
+    -> i >= f'
+    -> lab_approx symb L' LB
+    -> lab_approx (drop (i -f') symb) (drop (i -f') L') (drop (i -f') LB).
+Proof.
+  intros.
+  econstructor; intros. repeat rewrite drop_drop.
+  eapply get_drop in H3.
+  eapply get_drop in H4.
+  inv H2; exploit LEQ; eauto; dcr; clear LEQ.
+  exploit (sawtooth_resetting ST _ H H3); eauto. simpl in *.
+  orewrite (i0 - f'0 + (i - f') = (i - f') + i0 - f'0).
+  split; eauto. split; eauto.
+  orewrite (i0 - f'0 + length F0 + (i - f') = i - f' + i0 - f'0 + length F0). eauto.
+  split; eauto.
+  split; eauto.
+  inv H2; clear LEQ.
+  eapply sawtooth_drop in H; eauto.
+Qed.
+
+
+
+Inductive labIndicesSim : I.state -> IL.I.state -> Prop :=
+  | labIndicesSimI (L:env (option I.block)) L' E s s' symb LB
+    (EQ:labIndices symb s = Success s')
+    (LA:lab_approx symb L' LB)
+(*    (LL:forall l b, L (counted l) = Some b -> fst (fst (I.block_F b)) = l) *)
+    (EX:forall f i k, pos symb f k = Some i -> exists blk, L f = Some blk)
+    (*    (SM:forall l blk, L l = Some blk -> I.block_f blk < length (I.block_F blk)) *)
+    (BL:forall f blk, L f = Some blk -> exists j, pos symb f 0 = Some j /\
+                                        get LB j blk)
+    : labIndicesSim (L, E, s) (L', E, s').
+
+Lemma labIndicesSim_sim σ1 σ2
+  : labIndicesSim σ1 σ2 -> bisim σ1 σ2.
+Proof.
+  revert σ1 σ2. cofix; intros.
+  destruct H; destruct s; simpl in *; try monadS_inv EQ.
+  - case_eq (exp_eval E e); intros.
+    + one_step. eapply labIndicesSim_sim; econstructor; eauto.
+    + no_step.
+  - case_eq (exp_eval E e); intros.
+    case_eq (val2bool v); intros; one_step; eapply labIndicesSim_sim; econstructor; eauto.
+    no_step.
+  - eapply option2status_inv in EQ0.
+    edestruct EX as [[Lb F f]]; eauto. intros.
+    edestruct BL as [i [A B]]; eauto.
+    inv LA. edestruct (pos_get_first _ _ _ EQ0); dcr; eauto.
+    symmetry in H3; invc H3.
+    assert (x = i) by congruence; subst; clear_dup.
+    orewrite (i - 0 = i) in H1.
+    edestruct LEQ as [C2 [C3 [[Z [s C4]] [C5 [C6 [C7 C8]]]]]]; eauto.
+    decide (length Z = length Y).
+    case_eq (omap (exp_eval E) Y); intros.
+    edestruct C5 as [s' [D1 [D2 D3]]]; eauto.
+    {
+      edestruct C6.
+      intros. eapply H5. instantiate (1:=i - f + n). omega.
+      eapply get_drop. rewrite H3.
+      eapply get_app. eapply (map_get_1 (fst ∘ fst) H6).
+    }
+    + one_step. orewrite (l + 0 = l). eauto. simpl.
+      eapply get_drop in D1; eauto.
+      orewrite (i - f + f = i) in D1. eauto.
+      simpl. congruence.
+      eapply labIndicesSim_sim.
+      econstructor; eauto. simpl.
+      * eapply lab_approx_drop; eauto.
+      * intros.
+        decide (f0 ∈ of_list (List.map (fst ∘ fst) F)).
+        eapply update_with_list_lookup_in_list in i1. dcr.
+        erewrite H7. simpl in *. inv_map H4. eauto. eauto with len.
+        erewrite (update_with_list_no_update _ _ _ n); eauto.
+        destruct C6. rewrite H4 in H3.
+        rewrite pos_app_not_in in H3.
+        eapply C3. rewrite Plus.plus_comm. rewrite <- drop_drop. rewrite H4.
+        erewrite <- map_length. erewrite drop_length_eq. eauto. eauto.
+      * intros. destruct C6; subst. rewrite H4.
+        decide (f0 ∈ of_list (List.map (fst ∘ fst) F)).
+        edestruct (of_list_get_first _ i0) as [n]; eauto. dcr. hnf in H7. subst x0.
+        rewrite pos_app_in; eauto.
+        pose proof H8.
+        eapply update_with_list_lookup_in_list_first in H8; dcr.
+        erewrite H12 in H3. subst x0.
+        eexists; split. eapply get_first_pos; eauto.
+        rewrite H6. eapply get_app.
+        inv_map H11; eauto.
+        eauto with len.
+        eauto.
+        erewrite (update_with_list_no_update _ _ _ n) in H3; eauto.
+        edestruct C2; eauto; dcr.
+        rewrite H4 in H7. eexists; eauto.
+    +  intros. no_step.
+    +  no_step.
+       rewrite Ldef in H. inv H. simpl in *. repeat get_functional; subst. eauto.
+       repeat get_functional; subst. eauto.
+       edestruct C5; eauto; dcr. simpl in *.
+       intros. eapply H5. instantiate (1:=i - f + n0). omega.
+       eapply get_drop. rewrite H3.
+       eapply get_app. eapply (map_get_1 (fst ∘ fst) H6).
+       eapply get_drop in H3. orewrite (i - f + f = i) in H3.
+       get_functional; subst. simpl in *. congruence.
+  - no_step.
+  - case_eq (omap (exp_eval E) Y); intros.
+    + extern_step.
+      * eexists (ExternI f l default_val); eexists; try (now (econstructor; eauto)).
+      * eapply labIndicesSim_sim; econstructor; eauto.
+      * eapply labIndicesSim_sim; econstructor; eauto.
+    + no_step.
+  - one_step. eapply labIndicesSim_sim. econstructor; eauto.
+    instantiate (1:=(mapi (I.mkBlock L F) F ++ LB)).
+    econstructor. intros.
+    eapply get_app_cases in H. destruct H.
+    * {
+        inv_mapi H.
+        exploit @get_length; eauto. rewrite mapi_length in H2.
+        eapply get_in_range_app in H0.
+        orewrite (f' - f' = 0); simpl.
+        split.
+        - intros. edestruct BL; eauto; dcr.
+          eexists (length F0 + x2); split.
+          rewrite pos_app_not_in; eauto.
+          rewrite map_length. eapply pos_add; eauto.
+          eapply get_app_right.
+          rewrite mapi_length. reflexivity. eauto.
+        - split. intros. erewrite <- map_length in H3.
+          rewrite drop_length_eq in H3.
+          eapply EX; eauto.
+          split; eauto. destruct x1 as [[? ?] ?].
+          inv_map H0; unfold comp in *; simpl in *.
+          do 2 eexists; eauto.
+          split; eauto.
+          intros. eapply smap_spec in EQ0; eauto; dcr. destruct EQ0; dcr.
+          monadS_inv H6. simpl in *. eexists. repeat split; eauto.
+          eapply get_app.
+          intros.
+          eapply (mapi_get_1 0 (IL.I.mkBlock)) in H7. eauto.
+          assert (get (List.map (fst ∘ fst) F0) fn fb).
+          eapply (map_get_1 (fst ∘ fst) H3).
+          rewrite pos_app_in.
+          eapply get_first_pos; eauto.
+          intros. inv_map H8. eapply H4; eauto.
+          eapply get_in_of_list; eauto.
+          split; eauto.
+        - eauto with len.
+      }
+    * dcr.
+      assert (length (List.map (fst ∘ fst) F) = length (mapi (I.mkBlock L F) F)) by eauto with len.
+      assert (length F = length (mapi (I.mkBlock L F) F)) by eauto with len.
+      orewrite (i =  length (List.map (fst ∘ fst) F) + (i -  length (mapi (I.mkBlock L F) F))) in H0.
+      eapply shift_get in H0.
+      inv LA; exploit LEQ; eauto; dcr; clear LEQ.
+      orewrite (i - f' = i - length (mapi (I.mkBlock L F) F) - f' + length (mapi (I.mkBlock L F) F)).
+      split.
+      repeat rewrite <- drop_drop. repeat rewrite drop_length_eq.
+
+      intros.
+      setoid_rewrite <- H at 2.
+      rewrite drop_length_eq. eauto.
+      split; eauto.
+      orewrite (i - length (mapi (I.mkBlock L F) F) - f' + length (mapi (I.mkBlock L F) F) +
+         length F0 = i - length (mapi (I.mkBlock L F) F) - f' +
+                     length F0 + length (mapi (I.mkBlock L F) F)).
+      setoid_rewrite <- H at 2.
+      rewrite <- drop_drop. rewrite drop_length_eq. eauto.
+      split; eauto.
+      rewrite <- drop_drop.
+      eapply smap_length in EQ0.
+      repeat rewrite mapi_length.
+      repeat rewrite mapi_length in *.
+      repeat rewrite drop_drop.
+      repeat rewrite drop_app_gen. repeat rewrite mapi_length. repeat rewrite map_length.
+      assert (PLUSEQ: forall x y, x + y -y = x) by (intros; omega).
+      rewrite EQ0. repeat rewrite PLUSEQ. split; eauto.
+      split; eauto. split; eauto. omega.
+      rewrite mapi_length; omega.
+      rewrite map_length. omega.
+      rewrite mapi_length; omega.
+    * { inv LA. revert ST. clear_all.
+        intros. econstructor; eauto.
+        unfold mapi. generalize 0. generalize F at 1.
+        general induction F; simpl; eauto.
+        econstructor.
+        econstructor. eapply IHF. econstructor; simpl. reflexivity.
+      }
+    * {
+        intros.
+        decide (f ∈ of_list (List.map (fst ∘ fst) F)).
+        - eapply update_with_list_lookup_in_list in i0. dcr.
+          rewrite H2. simpl in *. inv_map H0. eauto.
+          eauto with len.
+        -  erewrite (update_with_list_no_update _ _ _ n); eauto.
+           rewrite pos_app_not_in in H; eauto.
+      }
+    * { intros.
+        decide (f ∈ of_list (List.map (fst ∘ fst) F)).
+        - edestruct (of_list_get_first _ i) as [n]; eauto. dcr. hnf in H1. subst x1.
+          rewrite pos_app_in; eauto.
+          pose proof H2.
+          eapply update_with_list_lookup_in_list_first in H0; dcr.
+          erewrite H5 in H. subst x1.
+          erewrite get_first_pos; eauto.
+          eexists; split; eauto.
+          inv_map H3. eapply get_app; eauto.
+          eauto with len.
+          eauto.
+        - erewrite update_with_list_no_update in H; eauto.
+          edestruct BL; eauto; dcr.
+          eexists; split; eauto using get_shift.
+          repeat rewrite pos_app_not_in; eauto.
+          assert (length (List.map (fst ∘ fst) F) = length (mapi (I.mkBlock L F) F))
+                 by eauto with len.
+          rewrite H0. eapply pos_add; eauto.
+      }
+Qed.
